Factor NN defs through common module

theories/MaxOfTwoNumbers/Model.v
@@ -2,7 +2,7 @@ From Coq Require Import Floats Sint63 Uint63 QArith Lia List PArray Morphisms Re
 From NeuralNetInterp.Util Require Import Default Pointed PArray List Notations Arith.Classes Arith.Instances Bool Option.
 From NeuralNetInterp.Util Require Nat Wf_Uint63.
 From NeuralNetInterp.Torch Require Import Tensor Einsum Slicing.
-From NeuralNetInterp.TransformerLens Require Import HookedTransformer HookedTransformer.Config.
+From NeuralNetInterp.TransformerLens Require Import HookedTransformer HookedTransformer.Config HookedTransformer.Module.
 From NeuralNetInterp.MaxOfTwoNumbers Require Import Parameters.
 Import Util.Nat.Notations.
 Import Util.Wf_Uint63.LoopNotation.
@@ -44,137 +44,74 @@ Module Import cfg <: Config.
           , L0_ln1_w, L0_ln1_b)].
 End cfg.
 
-Definition all_tokens : tensor [(cfg.d_vocab ^ cfg.n_ctx)%core : N; 2] RawIndexType
-  := let all_toks := Tensor.arange (start:=0) (Uint63.of_Z cfg.d_vocab) in
-     PArray.checkpoint (Tensor.cartesian_prod all_toks all_toks).
+Module Export Model.
+  Include Model cfg.
+  Export HookedTransformer.
 
-Section with_batch.
-  Context {r} {batch : Shape r} {pos}
-    (s := (batch ::' pos)%shape)
-    (resid_shape := (s ::' cfg.d_model)%shape)
-    {return_per_token : with_default "return_per_token" bool false}
-    {A} {coer_float : has_coer float A} {coerZ : has_coer Z A}
-    {zeroA : has_zero A} {oneA : has_one A}
-    (defaultA : pointed A := @coer _ _ coerZ point)
-    {addA : has_add A} {subA : has_sub A} {mulA : has_mul A} {divA : has_div A}
-    {ltbA : has_ltb A}
-    {oppA : has_opp A} {sqrtA : has_sqrt A} {expA : has_exp A} {lnA : has_ln A}
-    {use_checkpoint : with_default "use_checkpoint" bool true}.
-  #[local] Existing Instance defaultA.
-  #[local] Notation checkpoint x := (if use_checkpoint then PArray.checkpoint x else x%tensor).
+  Section with_batch.
+    Context {r} {batch : Shape r} {pos}
+      (s := (batch ::' pos)%shape)
+      (resid_shape := (s ::' cfg.d_model)%shape)
+      {return_per_token : with_default "return_per_token" bool false}
+      {A} {coer_float : has_coer float A} {coerZ : has_coer Z A}
+      (defaultA : pointed A := @coer _ _ coerZ point)
+      {addA : has_add A} {subA : has_sub A} {mulA : has_mul A} {divA : has_div A}
+      {ltbA : has_ltb A}
+      {oppA : has_opp A} {sqrtA : has_sqrt A} {expA : has_exp A} {lnA : has_ln A}
+      {use_checkpoint : with_default "use_checkpoint" bool true}.
+    #[local] Existing Instance defaultA.
+    #[local] Notation checkpoint x := (if use_checkpoint then PArray.checkpoint x else x%tensor).
 
-  Let coer_tensor_float {r s} (x : @tensor r s float) : @tensor r s A
-      := Tensor.map coer x.
-  Let coerA' (x : float) : A := coer x.
-  #[local] Set Warnings Append "-uniform-inheritance,-ambiguous-paths".
-  #[local] Coercion coer_tensor_float : tensor >-> tensor.
-  #[local] Set Warnings Append "uniform-inheritance,ambiguous-paths".
-  #[local] Coercion coerA' : float >-> A.
+    Let coer_tensor_float {r s} (x : @tensor r s float) : @tensor r s A
+        := Tensor.map coer x.
+    Let coerA' (x : float) : A := coer x.
+    #[local] Set Warnings Append "-uniform-inheritance,-ambiguous-paths".
+    #[local] Coercion coer_tensor_float : tensor >-> tensor.
+    #[local] Set Warnings Append "uniform-inheritance,ambiguous-paths".
+    #[local] Coercion coerA' : float >-> A.
 
-  Definition embed (tokens : tensor s IndexType) : tensor resid_shape A
-    := HookedTransformer.embed (A:=A) W_E tokens.
+    Definition masked_attn_scores (tokens : tensor s IndexType)
+        : tensor (batch ::' cfg.n_heads ::' pos ::' pos) A
+      := Option.invert_Some
+           (HookedTransformer.masked_attn_scores (A:=A) 0 tokens).
+    Definition attn_pattern (tokens : tensor s IndexType)
+        : tensor (batch ::' cfg.n_heads ::' pos ::' pos) A
+      := Option.invert_Some
+           (HookedTransformer.attn_pattern (A:=A) 0 tokens).
 
-  Definition pos_embed (tokens : tensor s IndexType) : tensor resid_shape A
-    := HookedTransformer.pos_embed (A:=A) (n_ctx:=cfg.n_ctx) W_pos tokens.
+    Definition loss_fn
+      (logits : tensor (s ::' cfg.d_vocab_out) A)
+      (tokens : tensor s IndexType)
+      : tensor (if return_per_token return Shape (if return_per_token then _ else _) then Shape.squeeze batch else []) A
+      := (let logits : tensor (batch ::' _) A
+            := checkpoint (logits.[…, -1, :]) in
+          let true_maximum : tensor (batch ::' 1) IndexType
+            := reduce_axis_m1 (keepdim:=true) Reduction.max tokens in
+          let log_probs
+            := log_softmax_dim_m1 logits in
+          let correct_log_probs
+            := checkpoint (gather_dim_m1 log_probs true_maximum) in
+          if return_per_token return (tensor (if return_per_token return Shape (if return_per_token then _ else _) then _ else _) A)
+          then -Tensor.squeeze correct_log_probs
+          else -Tensor.mean correct_log_probs)%core.
 
-  Definition ln_final (resid : tensor resid_shape A) : tensor resid_shape A
-    := HookedTransformer.ln_final (A:=A) cfg.eps ln_final_w ln_final_b resid.
-
-  Definition unembed (resid : tensor resid_shape A) : tensor (s ::' cfg.d_vocab_out) A
-    := HookedTransformer.unembed (A:=A) W_U b_U resid.
-
-  Definition blocks_params : list _
-    := [(L0_attn_W_Q:tensor _ A, L0_attn_W_K:tensor _ A, L0_attn_W_V:tensor _ A, L0_attn_W_O:tensor _ A,
-          L0_attn_b_Q:tensor _ A, L0_attn_b_K:tensor _ A, L0_attn_b_V:tensor _ A,
-          L0_attn_b_O:tensor _ A,
-          L0_ln1_w:tensor _ A, L0_ln1_b:tensor _ A)].
-
-  Definition logits (tokens : tensor s IndexType) : tensor (s ::' cfg.d_vocab_out) A
-    := HookedTransformer.logits
-         (A:=A)
-         (n_ctx:=cfg.n_ctx)
-         cfg.eps
-         W_E
-         W_pos
-
-         blocks_params
-
-         ln_final_w ln_final_b
-
-         W_U b_U
-
-         tokens.
-
-  (** convenience *)
-  Definition masked_attn_scores (tokens : tensor s IndexType)
-    : tensor (batch ::' cfg.n_heads ::' pos ::' pos) A
-    := Option.invert_Some
-         (HookedTransformer.HookedTransformer.masked_attn_scores
-            (A:=A)
-            (n_ctx:=cfg.n_ctx)
-            cfg.eps
-            W_E
-            W_pos
-
-            blocks_params
-
-            0
-
-            tokens).
-
-  Definition attn_pattern (tokens : tensor s IndexType)
-    : tensor (batch ::' cfg.n_heads ::' pos ::' pos) A
-    := Option.invert_Some
-         (HookedTransformer.HookedTransformer.attn_pattern
-            (A:=A)
-            (n_ctx:=cfg.n_ctx)
-            cfg.eps
-            W_E
-            W_pos
-
-            blocks_params
-
-            0
-
-            tokens).
-
-  Definition loss_fn
-    (logits : tensor (s ::' cfg.d_vocab_out) A)
-    (tokens : tensor s IndexType)
-  : tensor (if return_per_token return Shape (if return_per_token then _ else _) then Shape.squeeze batch else []) A
-  := (let logits : tensor (batch ::' _) A
-        := checkpoint (logits.[…, -1, :]) in
-      let true_maximum : tensor (batch ::' 1) IndexType
-        := reduce_axis_m1 (keepdim:=true) Reduction.max tokens in
-      let log_probs
-        := log_softmax_dim_m1 logits in
-      let correct_log_probs
-        := checkpoint (gather_dim_m1 log_probs true_maximum) in
-      if return_per_token return (tensor (if return_per_token return Shape (if return_per_token then _ else _) then _ else _) A)
-      then -Tensor.squeeze correct_log_probs
-      else -Tensor.mean correct_log_probs)%core.
-
-  Definition acc_fn
-    (logits : tensor (s ::' cfg.d_vocab_out) A)
-    (tokens : tensor s IndexType)
-    : tensor (if return_per_token return Shape (if return_per_token then _ else _) then batch else []) A
-    := (let pred_logits : tensor (batch ::' _) A
-          := checkpoint (logits.[…, -1, :]) in
-        let pred_tokens : tensor batch IndexType
-          := reduce_axis_m1 (keepdim:=false) Reduction.argmax pred_logits in
-        let true_maximum : tensor batch IndexType
-          := reduce_axis_m1 (keepdim:=false) Reduction.max tokens in
-        let res : tensor _ A
-          := checkpoint (Tensor.of_bool (Tensor.map2 eqb pred_tokens true_maximum)) in
-        if return_per_token return (tensor (if return_per_token return Shape (if return_per_token then _ else _) then _ else _) A)
-        then res
-        else Tensor.mean res)%core.
-End with_batch.
-
-Notation model := logits (only parsing).
-
-Definition logits_all_tokens : tensor _ float
-  := logits all_tokens.
+    Definition acc_fn
+      (logits : tensor (s ::' cfg.d_vocab_out) A)
+      (tokens : tensor s IndexType)
+      : tensor (if return_per_token return Shape (if return_per_token then _ else _) then batch else []) A
+      := (let pred_logits : tensor (batch ::' _) A
+            := checkpoint (logits.[…, -1, :]) in
+          let pred_tokens : tensor batch IndexType
+            := reduce_axis_m1 (keepdim:=false) Reduction.argmax pred_logits in
+          let true_maximum : tensor batch IndexType
+            := reduce_axis_m1 (keepdim:=false) Reduction.max tokens in
+          let res : tensor _ A
+            := checkpoint (Tensor.of_bool (Tensor.map2 eqb pred_tokens true_maximum)) in
+          if return_per_token return (tensor (if return_per_token return Shape (if return_per_token then _ else _) then _ else _) A)
+          then res
+          else Tensor.mean res)%core.
+  End with_batch.
+End Model.
 
 (*
 Definition expected : tensor _ _ := Eval cbv in tensor_of_list [[11.4344;  0.5226;  3.3839;  1.9724;  4.5840;  0.6439;  3.9603;
