theories/MaxOfTwoNumbersSimpler/Model.v
@@ -2,8 +2,8 @@ From Coq Require Import Floats Sint63 Uint63 QArith Lia List PArray Morphisms Re
 From NeuralNetInterp.Util Require Import Default Pointed PArray List Notations Arith.Classes Arith.Instances Bool Option.
 From NeuralNetInterp.Util Require Nat Wf_Uint63.
 From NeuralNetInterp.Torch Require Import Tensor Einsum Slicing.
-From NeuralNetInterp.TransformerLens Require Import HookedTransformer.
-From NeuralNetInterp.MaxOfTwoNumbers Require Import Parameters.
+From NeuralNetInterp.TransformerLens Require Import HookedTransformer HookedTransformer.Config HookedTransformer.Module.
+From NeuralNetInterp.MaxOfTwoNumbersSimpler Require Import Parameters.
 Import Util.Nat.Notations.
 Import Util.Wf_Uint63.LoopNotation.
 Import Util.Wf_Uint63.
@@ -18,164 +18,95 @@ Local Open Scope raw_tensor_scope.
 
 (* Based on https://colab.research.google.com/drive/1N4iPEyBVuctveCA0Zre92SpfgH6nmHXY#scrollTo=Q1h45HnKi-43, Taking the minimum or maximum of two ints *)
 
-(** Hyperparameters *)
-Definition N_LAYERS : nat := 1.
-Definition N_HEADS : nat := 1.
-Definition D_MODEL : nat := 32.
-Definition D_HEAD : nat := 32.
-(*Definition D_MLP = None*)
+Module Import cfg <: Config.
+  Include Parameters.cfg.
 
-Definition D_VOCAB : nat := 64.
+  Definition W_E : tensor _ _ := Eval cbv in tensor_of_list Parameters.W_E.
+  Definition W_pos : tensor _ _ := Eval cbv in tensor_of_list Parameters.W_pos.
+  Definition L0_attn_W_Q : tensor _ _ := Eval cbv in tensor_of_list Parameters.L0_attn_W_Q.
+  Definition L0_attn_W_K : tensor _ _ := Eval cbv in tensor_of_list Parameters.L0_attn_W_K.
+  Definition L0_attn_W_V : tensor _ _ := Eval cbv in tensor_of_list Parameters.L0_attn_W_V.
+  Definition L0_attn_W_O : tensor _ _ := Eval cbv in tensor_of_list Parameters.L0_attn_W_O.
+  Definition L0_attn_b_Q : tensor _ _ := Eval cbv in tensor_of_list Parameters.L0_attn_b_Q.
+  Definition L0_attn_b_K : tensor _ _ := Eval cbv in tensor_of_list Parameters.L0_attn_b_K.
+  Definition L0_attn_b_V : tensor _ _ := Eval cbv in tensor_of_list Parameters.L0_attn_b_V.
+  Definition L0_attn_b_O : tensor _ _ := Eval cbv in tensor_of_list Parameters.L0_attn_b_O.
+  Definition ln_final_b := I.
+  Definition ln_final_w := I.
+  Definition W_U : tensor _ _ := Eval cbv in tensor_of_list Parameters.W_U.
+  Definition b_U : tensor _ _ := Eval cbv in tensor_of_list Parameters.b_U.
 
-Notation tensor_of_list ls := (Tensor.PArray.abstract (Tensor.PArray.concretize (Tensor.of_list ls))) (only parsing).
-Definition W_E : tensor _ _ := Eval cbv in tensor_of_list MaxOfTwoNumbers.Parameters.W_E.
-Definition W_pos : tensor _ _ := Eval cbv in tensor_of_list MaxOfTwoNumbers.Parameters.W_pos.
-Definition L0_attn_W_Q : tensor _ _ := Eval cbv in tensor_of_list MaxOfTwoNumbers.Parameters.L0_attn_W_Q.
-Definition L0_attn_W_K : tensor _ _ := Eval cbv in tensor_of_list MaxOfTwoNumbers.Parameters.L0_attn_W_K.
-Definition L0_attn_W_V : tensor _ _ := Eval cbv in tensor_of_list MaxOfTwoNumbers.Parameters.L0_attn_W_V.
-Definition L0_attn_W_O : tensor _ _ := Eval cbv in tensor_of_list MaxOfTwoNumbers.Parameters.L0_attn_W_O.
-Definition L0_attn_b_Q : tensor _ _ := Eval cbv in tensor_of_list MaxOfTwoNumbers.Parameters.L0_attn_b_Q.
-Definition L0_attn_b_K : tensor _ _ := Eval cbv in tensor_of_list MaxOfTwoNumbers.Parameters.L0_attn_b_K.
-Definition L0_attn_b_V : tensor _ _ := Eval cbv in tensor_of_list MaxOfTwoNumbers.Parameters.L0_attn_b_V.
-Definition L0_attn_b_O : tensor _ _ := Eval cbv in tensor_of_list MaxOfTwoNumbers.Parameters.L0_attn_b_O.
-Definition L0_ln1_b : tensor _ _ := Eval cbv in tensor_of_list MaxOfTwoNumbers.Parameters.L0_ln1_b.
-Definition L0_ln1_w : tensor _ _ := Eval cbv in tensor_of_list MaxOfTwoNumbers.Parameters.L0_ln1_w.
-Definition ln_final_b : tensor _ _ := Eval cbv in tensor_of_list MaxOfTwoNumbers.Parameters.ln_final_b.
-Definition ln_final_w : tensor _ _ := Eval cbv in tensor_of_list MaxOfTwoNumbers.Parameters.ln_final_w.
-Definition W_U : tensor _ _ := Eval cbv in tensor_of_list MaxOfTwoNumbers.Parameters.W_U.
-Definition b_U : tensor _ _ := Eval cbv in tensor_of_list MaxOfTwoNumbers.Parameters.b_U.
+  Definition blocks_params
+    := [(L0_attn_W_Q, L0_attn_W_K, L0_attn_W_V, L0_attn_W_O
+          , L0_attn_b_Q, L0_attn_b_K, L0_attn_b_V, L0_attn_b_O
+          , I, I)].
+End cfg.
 
-Definition all_tokens : tensor [(cfg.d_vocab ^ cfg.n_ctx)%core : N; 2] RawIndexType
-  := let all_toks := Tensor.arange (start:=0) (Uint63.of_Z cfg.d_vocab) in
-     PArray.checkpoint (Tensor.cartesian_prod all_toks all_toks).
+Module Export Model.
+  Include Model cfg.
+  Export HookedTransformer.
 
-Section with_batch.
-  Context {r} {batch : Shape r} {pos}
-    (s := (batch ::' pos)%shape)
-    (resid_shape := (s ::' cfg.d_model)%shape)
-    {return_per_token : with_default "return_per_token" bool false}
-    {A} {coer_float : has_coer float A} {coerZ : has_coer Z A}
-    {zeroA : has_zero A} {oneA : has_one A}
-    (defaultA : pointed A := @coer _ _ coerZ point)
-    {addA : has_add A} {subA : has_sub A} {mulA : has_mul A} {divA : has_div A}
-    {ltbA : has_ltb A}
-    {oppA : has_opp A} {sqrtA : has_sqrt A} {expA : has_exp A} {lnA : has_ln A}
-    {use_checkpoint : with_default "use_checkpoint" bool true}.
-  #[local] Existing Instance defaultA.
-  #[local] Notation checkpoint x := (if use_checkpoint then PArray.checkpoint x else x%tensor).
+  Section with_batch.
+    Context {r} {batch : Shape r} {pos}
+      (s := (batch ::' pos)%shape)
+      (resid_shape := (s ::' cfg.d_model)%shape)
+      {return_per_token : with_default "return_per_token" bool false}
+      {A} {coer_float : has_coer float A} {coerZ : has_coer Z A}
+      (defaultA : pointed A := @coer _ _ coerZ point)
+      {addA : has_add A} {subA : has_sub A} {mulA : has_mul A} {divA : has_div A}
+      {ltbA : has_ltb A}
+      {oppA : has_opp A} {sqrtA : has_sqrt A} {expA : has_exp A} {lnA : has_ln A}
+      {use_checkpoint : with_default "use_checkpoint" bool true}.
+    #[local] Existing Instance defaultA.
+    #[local] Notation checkpoint x := (if use_checkpoint then PArray.checkpoint x else x%tensor).
 
-  Let coer_tensor_float {r s} (x : @tensor r s float) : @tensor r s A
-      := Tensor.map coer x.
-  Let coerA' (x : float) : A := coer x.
-  #[local] Set Warnings Append "-uniform-inheritance,-ambiguous-paths".
-  #[local] Coercion coer_tensor_float : tensor >-> tensor.
-  #[local] Set Warnings Append "uniform-inheritance,ambiguous-paths".
-  #[local] Coercion coerA' : float >-> A.
+    Let coer_tensor_float {r s} (x : @tensor r s float) : @tensor r s A
+        := Tensor.map coer x.
+    Let coerA' (x : float) : A := coer x.
+    #[local] Set Warnings Append "-uniform-inheritance,-ambiguous-paths".
+    #[local] Coercion coer_tensor_float : tensor >-> tensor.
+    #[local] Set Warnings Append "uniform-inheritance,ambiguous-paths".
+    #[local] Coercion coerA' : float >-> A.
 
-  Definition embed (tokens : tensor s IndexType) : tensor resid_shape A
-    := HookedTransformer.embed (A:=A) W_E tokens.
+    Definition masked_attn_scores (tokens : tensor s IndexType)
+        : tensor (batch ::' cfg.n_heads ::' pos ::' pos) A
+      := Option.invert_Some
+           (HookedTransformer.masked_attn_scores (A:=A) 0 tokens).
+    Definition attn_pattern (tokens : tensor s IndexType)
+        : tensor (batch ::' cfg.n_heads ::' pos ::' pos) A
+      := Option.invert_Some
+           (HookedTransformer.attn_pattern (A:=A) 0 tokens).
 
-  Definition pos_embed (tokens : tensor s IndexType) : tensor resid_shape A
-    := HookedTransformer.pos_embed (A:=A) (n_ctx:=cfg.n_ctx) W_pos tokens.
+    Definition loss_fn
+      (logits : tensor (s ::' cfg.d_vocab_out) A)
+      (tokens : tensor s IndexType)
+      : tensor (if return_per_token return Shape (if return_per_token then _ else _) then Shape.squeeze batch else []) A
+      := (let logits : tensor (batch ::' _) A
+            := checkpoint (logits.[…, -1, :]) in
+          let true_maximum : tensor (batch ::' 1) IndexType
+            := reduce_axis_m1 (keepdim:=true) Reduction.max tokens in
+          let log_probs
+            := log_softmax_dim_m1 logits in
+          let correct_log_probs
+            := checkpoint (gather_dim_m1 log_probs true_maximum) in
+          if return_per_token return (tensor (if return_per_token return Shape (if return_per_token then _ else _) then _ else _) A)
+          then -Tensor.squeeze correct_log_probs
+          else -Tensor.mean correct_log_probs)%core.
 
-  Definition ln_final (resid : tensor resid_shape A) : tensor resid_shape A
-    := HookedTransformer.ln_final (normalization_type:=None) (A:=A) cfg.eps I I resid.
-
-  Definition unembed (resid : tensor resid_shape A) : tensor (s ::' cfg.d_vocab_out) A
-    := HookedTransformer.unembed (A:=A) W_U b_U resid.
-
-  Definition blocks_params : list _
-    := [(L0_attn_W_Q:tensor _ A, L0_attn_W_K:tensor _ A, L0_attn_W_V:tensor _ A, L0_attn_W_O:tensor _ A,
-          L0_attn_b_Q:tensor _ A, L0_attn_b_K:tensor _ A, L0_attn_b_V:tensor _ A,
-          L0_attn_b_O:tensor _ A,
-          I, I)].
-
-  Definition logits (tokens : tensor s IndexType) : tensor (s ::' cfg.d_vocab_out) A
-    := HookedTransformer.logits
-         (A:=A)
-         (n_ctx:=cfg.n_ctx)
-         (normalization_type:=None)
-         cfg.eps
-         W_E
-         W_pos
-
-         blocks_params
-
-         I I
-
-         W_U b_U
-
-         tokens.
-
-  (** convenience *)
-  Definition masked_attn_scores (tokens : tensor s IndexType)
-    : tensor (batch ::' cfg.n_heads ::' pos ::' pos) A
-    := Option.invert_Some
-         (HookedTransformer.HookedTransformer.masked_attn_scores
-            (normalization_type:=None)
-            (A:=A)
-            (n_ctx:=cfg.n_ctx)
-            cfg.eps
-            W_E
-            W_pos
-
-            blocks_params
-
-            0
-
-            tokens).
-
-  Definition attn_pattern (tokens : tensor s IndexType)
-    : tensor (batch ::' cfg.n_heads ::' pos ::' pos) A
-    := Option.invert_Some
-         (HookedTransformer.HookedTransformer.attn_pattern
-            (normalization_type:=None)
-            (A:=A)
-            (n_ctx:=cfg.n_ctx)
-            cfg.eps
-            W_E
-            W_pos
-
-            blocks_params
-
-            0
-
-            tokens).
-
-  Definition loss_fn
-    (logits : tensor (s ::' cfg.d_vocab_out) A)
-    (tokens : tensor s IndexType)
-  : tensor (if return_per_token return Shape (if return_per_token then _ else _) then Shape.squeeze batch else []) A
-  := (let logits : tensor (batch ::' _) A
-        := checkpoint (logits.[…, -1, :]) in
-      let true_maximum : tensor (batch ::' 1) IndexType
-        := reduce_axis_m1 (keepdim:=true) Reduction.max tokens in
-      let log_probs
-        := log_softmax_dim_m1 logits in
-      let correct_log_probs
-        := checkpoint (gather_dim_m1 log_probs true_maximum) in
-      if return_per_token return (tensor (if return_per_token return Shape (if return_per_token then _ else _) then _ else _) A)
-      then -Tensor.squeeze correct_log_probs
-      else -Tensor.mean correct_log_probs)%core.
-
-  Definition acc_fn
-    (logits : tensor (s ::' cfg.d_vocab_out) A)
-    (tokens : tensor s IndexType)
-    : tensor (if return_per_token return Shape (if return_per_token then _ else _) then batch else []) A
-    := (let pred_logits : tensor (batch ::' _) A
-          := checkpoint (logits.[…, -1, :]) in
-        let pred_tokens : tensor batch IndexType
-          := reduce_axis_m1 (keepdim:=false) Reduction.argmax pred_logits in
-        let true_maximum : tensor batch IndexType
-          := reduce_axis_m1 (keepdim:=false) Reduction.max tokens in
-        let res : tensor _ A
-          := checkpoint (Tensor.of_bool (Tensor.map2 eqb pred_tokens true_maximum)) in
-        if return_per_token return (tensor (if return_per_token return Shape (if return_per_token then _ else _) then _ else _) A)
-        then res
-        else Tensor.mean res)%core.
-End with_batch.
-
-Notation model := logits (only parsing).
-
-Definition logits_all_tokens : tensor _ float
-  := logits all_tokens.
+    Definition acc_fn
+      (logits : tensor (s ::' cfg.d_vocab_out) A)
+      (tokens : tensor s IndexType)
+      : tensor (if return_per_token return Shape (if return_per_token then _ else _) then batch else []) A
+      := (let pred_logits : tensor (batch ::' _) A
+            := checkpoint (logits.[…, -1, :]) in
+          let pred_tokens : tensor batch IndexType
+            := reduce_axis_m1 (keepdim:=false) Reduction.argmax pred_logits in
+          let true_maximum : tensor batch IndexType
+            := reduce_axis_m1 (keepdim:=false) Reduction.max tokens in
+          let res : tensor _ A
+            := checkpoint (Tensor.of_bool (Tensor.map2 eqb pred_tokens true_maximum)) in
+          if return_per_token return (tensor (if return_per_token return Shape (if return_per_token then _ else _) then _ else _) A)
+          then res
+          else Tensor.mean res)%core.
+  End with_batch.
+End Model.
