theories/MaxOfTwoNumbersSimpler/Model/Instances.v
@@ -1,7 +1,7 @@
 From Coq Require Import Morphisms RelationClasses RelationPairs.
 From NeuralNetInterp.Util Require Import Default SolveProperEqRel Option.
-From NeuralNetInterp.Util.Tactics Require Import Head.
-From NeuralNetInterp.Util.List.Instances Require Import Forall2.
+From NeuralNetInterp.Util.Tactics Require Import Head DestructHead.
+From NeuralNetInterp.Util.List.Instances Require Import Forall2 Forall2.Map.
 From NeuralNetInterp.Torch Require Import Tensor Tensor.Instances Slicing Slicing.Instances.
 From NeuralNetInterp.TransformerLens Require Import HookedTransformer HookedTransformer.Instances.
 From NeuralNetInterp.MaxOfTwoNumbersSimpler Require Import Model.
@@ -43,7 +43,6 @@ Module Model.
     : Dependent.Proper
         ((Dependent.const eq ==> Dependent.idR)
            ==> (Dependent.const eq ==> Dependent.idR)
-           ==> Dependent.idR
            ==> (Dependent.idR ==> Dependent.idR ==> Dependent.idR)
            ==> (Dependent.idR ==> Dependent.idR ==> Dependent.idR)
            ==> (Dependent.idR ==> Dependent.idR ==> Dependent.idR)
@@ -53,16 +52,16 @@ Module Model.
            ==> Tensor.eqfR
            ==> Tensor.eqfR)
         (@ln_final r batch pos).
-  Proof. cbv [ln_final]; repeat intro; apply HookedTransformer.HookedTransformer.ln_final_Proper_dep; t. Qed.
+  Proof. cbv [ln_final cfg.normalization_type]; repeat intro; apply HookedTransformer.HookedTransformer.ln_final_Proper_dep; t. Qed.
 
-  #[export] Instance ln_final_Proper {r batch pos A coer_float coerZ zeroA addA subA mulA divA sqrtA use_checkpoint}
-    : Proper (Tensor.eqf ==> Tensor.eqf) (@ln_final r batch pos A coer_float coerZ zeroA addA subA mulA divA sqrtA use_checkpoint).
+  #[export] Instance ln_final_Proper {r batch pos A coer_float coerZ addA subA mulA divA sqrtA use_checkpoint}
+    : Proper (Tensor.eqf ==> Tensor.eqf) (@ln_final r batch pos A coer_float coerZ addA subA mulA divA sqrtA use_checkpoint).
   Proof. cbv [ln_final]; apply HookedTransformer.HookedTransformer.ln_final_Proper. Qed.
 
   #[export] Instance unembed_Proper_dep {r batch pos}
     : Dependent.Proper
         ((Dependent.const eq ==> Dependent.idR)
-           ==> Dependent.idR
+           ==> (Dependent.const eq ==> Dependent.idR)
            ==> (Dependent.idR ==> Dependent.idR ==> Dependent.idR)
            ==> (Dependent.idR ==> Dependent.idR ==> Dependent.idR)
            ==> Tensor.eqfR
@@ -70,39 +69,46 @@ Module Model.
         (@unembed r batch pos).
   Proof. cbv [unembed]; repeat intro; apply HookedTransformer.HookedTransformer.unembed_Proper_dep; t. Qed.
 
-  #[export] Instance unembed_Proper {r batch pos A coer_float zeroA addA mulA}
-    : Proper (Tensor.eqf ==> Tensor.eqf) (@unembed r batch pos A coer_float zeroA addA mulA).
+  #[export] Instance unembed_Proper {r batch pos A coer_float coerZ addA mulA}
+    : Proper (Tensor.eqf ==> Tensor.eqf) (@unembed r batch pos A coer_float coerZ addA mulA).
   Proof. cbv [unembed]; apply HookedTransformer.HookedTransformer.unembed_Proper. Qed.
 
-  #[export] Instance blocks_params_Proper_dep
-    : Dependent.Proper
-        ((Dependent.const eq ==> Dependent.idR)
-           ==> List.Forall2 ∘ (Tensor.eqfR * Tensor.eqfR
-                               * Tensor.eqfR * Tensor.eqfR
-                               * Tensor.eqfR * Tensor.eqfR
-                               * Tensor.eqfR * Tensor.eqfR
-                               * Dependent.const (@eq True) * Dependent.const (@eq True)))
-        (@blocks_params).
-  Proof.
-    cbv [blocks_params]; repeat intro; repeat constructor; cbv [Dependent.RelCompFun]; cbn [fst snd].
-    all: eapply Tensor.map_Proper_dep; try eassumption.
-    all: repeat intro; reflexivity.
-  Qed.
-
-  #[export] Instance blocks_params_Proper {A coer_float}
+  #[export] Instance blocks_params_Proper
     : Proper (List.Forall2 (Tensor.eqf * Tensor.eqf
                             * Tensor.eqf * Tensor.eqf
                             * Tensor.eqf * Tensor.eqf
                             * Tensor.eqf * Tensor.eqf
                             * @eq True * @eq True)%signature)
-        (@blocks_params A coer_float).
-  Proof. apply blocks_params_Proper_dep; repeat intro; subst; reflexivity. Qed.
+        (@cfg.blocks_params).
+  Proof. hnf; apply reflexivity. Qed.
+
+  #[export] Instance coer_blocks_params_Proper_dep
+    : Dependent.Proper
+        ((Dependent.const eq ==> Dependent.idR)
+           ==> Dependent.const (List.Forall2 (Tensor.eqf * Tensor.eqf
+                                              * Tensor.eqf * Tensor.eqf
+                                              * Tensor.eqf * Tensor.eqf
+                                              * Tensor.eqf * Tensor.eqf
+                                              * @eq True * @eq True)%signature)
+           ==> List.Forall2 ∘ (Tensor.eqfR * Tensor.eqfR
+                               * Tensor.eqfR * Tensor.eqfR
+                               * Tensor.eqfR * Tensor.eqfR
+                               * Tensor.eqfR * Tensor.eqfR
+                               * Dependent.const (@eq True) * Dependent.const (@eq True)))
+        (@coer_blocks_params).
+  Proof.
+    cbv [coer_blocks_params cfg.normalization_type]; t.
+    eapply List.map_Proper_dep; try eassumption; [].
+    repeat intro; destruct_head'_prod.
+    cbv [Dependent.lift2_1 Dependent.lift2_2 Dependent.RelProd Dependent.relation_conjunction Dependent.RelCompFun RelProd RelCompFun relation_conjunction predicate_intersection pointwise_extension] in *; cbn [fst snd] in *.
+    destruct_head'_and.
+    repeat apply conj; t.
+  Qed.
 
   #[export] Instance logits_Proper_dep {r batch pos}
     : Dependent.Proper
         ((Dependent.const eq ==> Dependent.idR)
            ==> (Dependent.const eq ==> Dependent.idR)
-           ==> Dependent.idR
            ==> (Dependent.idR ==> Dependent.idR ==> Dependent.idR)
            ==> (Dependent.idR ==> Dependent.idR ==> Dependent.idR)
            ==> (Dependent.idR ==> Dependent.idR ==> Dependent.idR)
@@ -113,17 +119,16 @@ Module Model.
            ==> Dependent.const Tensor.eqf
            ==> Tensor.eqfR)
         (@logits r batch pos).
-  Proof. cbv [logits]; repeat intro; apply HookedTransformer.HookedTransformer.logits_Proper_dep; try apply blocks_params_Proper_dep; t. Qed.
+  Proof. cbv [logits cfg.normalization_type]; repeat intro; apply HookedTransformer.HookedTransformer.logits_Proper_dep; try apply coer_blocks_params_Proper_dep; t. Qed.
 
-  #[export] Instance logits_Proper {r batch pos A coer_float coerZ zeroA addA subA mulA divA sqrtA expA use_checkpoint}
-    : Proper (Tensor.eqf ==> Tensor.eqf) (@logits r batch pos A coer_float coerZ zeroA addA subA mulA divA sqrtA expA use_checkpoint)
+  #[export] Instance logits_Proper {r batch pos A coer_float coerZ addA subA mulA divA sqrtA expA use_checkpoint}
+    : Proper (Tensor.eqf ==> Tensor.eqf) (@logits r batch pos A coer_float coerZ addA subA mulA divA sqrtA expA use_checkpoint)
     := HookedTransformer.HookedTransformer.logits_Proper.
 
   #[export] Instance masked_attn_scores_Proper_dep {r batch pos}
     : Dependent.Proper
         ((Dependent.const eq ==> Dependent.idR)
            ==> (Dependent.const eq ==> Dependent.idR)
-           ==> Dependent.idR
            ==> (Dependent.idR ==> Dependent.idR ==> Dependent.idR)
            ==> (Dependent.idR ==> Dependent.idR ==> Dependent.idR)
            ==> (Dependent.idR ==> Dependent.idR ==> Dependent.idR)
@@ -149,18 +154,17 @@ Module Model.
     end.
     Unshelve.
     all: cbv beta iota; t.
-    all: try apply blocks_params_Proper_dep; t.
+    all: try apply coer_blocks_params_Proper_dep; t.
   Qed.
 
-  #[export] Instance masked_attn_scores_Proper {r batch pos A coer_float coerZ zeroA addA subA mulA divA sqrtA expA use_checkpoint}
-    : Proper (Tensor.eqf ==> Tensor.eqf) (@masked_attn_scores r batch pos A coer_float coerZ zeroA addA subA mulA divA sqrtA expA use_checkpoint).
+  #[export] Instance masked_attn_scores_Proper {r batch pos A coer_float coerZ addA subA mulA divA sqrtA expA use_checkpoint}
+    : Proper (Tensor.eqf ==> Tensor.eqf) (@masked_attn_scores r batch pos A coer_float coerZ addA subA mulA divA sqrtA expA use_checkpoint).
   Proof. apply masked_attn_scores_Proper_dep; repeat intro; subst; reflexivity. Qed.
 
   #[export] Instance attn_pattern_Proper_dep {r batch pos}
     : Dependent.Proper
         ((Dependent.const eq ==> Dependent.idR)
            ==> (Dependent.const eq ==> Dependent.idR)
-           ==> Dependent.idR
            ==> (Dependent.idR ==> Dependent.idR ==> Dependent.idR)
            ==> (Dependent.idR ==> Dependent.idR ==> Dependent.idR)
            ==> (Dependent.idR ==> Dependent.idR ==> Dependent.idR)
@@ -186,11 +190,11 @@ Module Model.
     end.
     Unshelve.
     all: cbv beta iota; t.
-    all: try apply blocks_params_Proper_dep; t.
+    all: try apply coer_blocks_params_Proper_dep; t.
   Qed.
 
-  #[export] Instance attn_pattern_Proper {r batch pos A coer_float coerZ zeroA addA subA mulA divA sqrtA expA use_checkpoint}
-    : Proper (Tensor.eqf ==> Tensor.eqf) (@attn_pattern r batch pos A coer_float coerZ zeroA addA subA mulA divA sqrtA expA use_checkpoint).
+  #[export] Instance attn_pattern_Proper {r batch pos A coer_float coerZ addA subA mulA divA sqrtA expA use_checkpoint}
+    : Proper (Tensor.eqf ==> Tensor.eqf) (@attn_pattern r batch pos A coer_float coerZ addA subA mulA divA sqrtA expA use_checkpoint).
   Proof. apply attn_pattern_Proper_dep; repeat intro; subst; reflexivity. Qed.
 
   Notation model_Proper := logits_Proper (only parsing).
@@ -198,7 +202,6 @@ Module Model.
   #[export] Instance loss_fn_Proper_dep {r batch pos return_per_token}
     : Dependent.Proper
         ((Dependent.const eq ==> Dependent.idR)
-           ==> Dependent.idR
            ==> (Dependent.idR ==> Dependent.idR ==> Dependent.idR)
            ==> (Dependent.idR ==> Dependent.idR ==> Dependent.idR)
            ==> (Dependent.idR ==> Dependent.idR)
@@ -211,15 +214,13 @@ Module Model.
         (@loss_fn r batch pos return_per_token).
   Proof. cbv [loss_fn]; HookedTransformer.t. Qed.
 
-  #[export] Instance loss_fn_Proper {r batch pos return_per_token A coerZ zeroA addA divA oppA expA lnA use_checkpoint}
-    : Proper (Tensor.eqf ==> Tensor.eqf ==> Tensor.eqf) (@loss_fn r batch pos return_per_token A coerZ zeroA addA divA oppA expA lnA use_checkpoint).
+  #[export] Instance loss_fn_Proper {r batch pos return_per_token A coerZ addA divA oppA expA lnA use_checkpoint}
+    : Proper (Tensor.eqf ==> Tensor.eqf ==> Tensor.eqf) (@loss_fn r batch pos return_per_token A coerZ addA divA oppA expA lnA use_checkpoint).
   Proof. apply loss_fn_Proper_dep; repeat intro; subst; reflexivity. Qed.
 
   #[export] Instance acc_fn_Proper_dep {r batch pos return_per_token}
     : Dependent.Proper
         ((Dependent.const eq ==> Dependent.idR)
-           ==> Dependent.idR
-           ==> Dependent.idR
            ==> (Dependent.idR ==> Dependent.idR ==> Dependent.idR)
            ==> (Dependent.idR ==> Dependent.idR ==> Dependent.idR)
            ==> (Dependent.idR ==> Dependent.idR ==> Dependent.const eq)
@@ -230,8 +231,8 @@ Module Model.
         (@acc_fn r batch pos return_per_token).
   Proof. cbv [acc_fn]; HookedTransformer.t; try (subst; reflexivity). Qed.
 
-  #[export] Instance acc_fn_Proper {r batch pos return_per_token A coerZ zeroA oneA addA divA ltbA use_checkpoint}
-    : Proper (Tensor.eqf ==> Tensor.eqf ==> Tensor.eqf) (@acc_fn r batch pos return_per_token A coerZ zeroA oneA addA divA ltbA use_checkpoint).
+  #[export] Instance acc_fn_Proper {r batch pos return_per_token A coerZ addA divA ltbA use_checkpoint}
+    : Proper (Tensor.eqf ==> Tensor.eqf ==> Tensor.eqf) (@acc_fn r batch pos return_per_token A coerZ addA divA ltbA use_checkpoint).
   Proof. apply acc_fn_Proper_dep; repeat intro; subst; reflexivity. Qed.
 End Model.
 Export (hints) Model.
