theories/Util/List/Forall2Map.v
@@ -1,0 +1,12 @@
+From Coq Require Import List.
+Import ListNotations.
+#[local] Open Scope list_scope.
+
+Module List.
+  Lemma Forall2_map {A B A' B' f g P xs ys}
+    : @Forall2 A' B' P (map f xs) (map g ys) <-> @Forall2 A B (fun x y => P (f x) (g y)) xs ys.
+  Proof.
+    split; revert ys; induction xs as [|x xs IH], ys as [|y ys]; cbn [map]; intro H;
+      inversion H; clear H; subst; constructor; eauto.
+  Qed.
+End List.
