theories/Util/List/Instances/Forall2/Map.v
@@ -1,0 +1,18 @@
+From Coq Require Import Morphisms RelationClasses RelationPairs List.
+From NeuralNetInterp.Util.List Require Import Forall2Map.
+From NeuralNetInterp.Util Require Import Morphisms.Dependent RelationClasses.Dependent Program.Basics.Dependent.
+Import Dependent.ProperNotations.
+
+Module List.
+  #[export] Instance map_Proper_dep
+  : Dependent.Proper2
+      ((Dependent.lift2_1 Dependent.idR ==> Dependent.lift2_2 Dependent.idR)
+         ==> Dependent.lift2_1 (List.Forall2 ∘ Dependent.idR)
+         ==> Dependent.lift2_2 (List.Forall2 ∘ Dependent.idR))
+      (@List.map).
+  Proof.
+    cbv -[List.map]; intros; rewrite List.Forall2_map.
+    eapply Forall2_impl; [ | eassumption ]; eauto.
+  Qed.
+End List.
+Export (hints) List.
